### Inner Product
Usual $\left< \psi,\phi \right>=\int \psi^*\phi$. Then the conjugate $\hat Q^*$ of $Q$ satisfies $\left< \phi,\hat{Q}\psi \right> =\left< \hat{Q}^*\phi,\psi \right>$. Then $\hat{Q}$ is Hermitian iff. $\hat{Q}=\hat{Q}^*$.

>[!important] Copenhagen Measurement Postulate
> Given $\left< \phi,\phi \right> =1,$ the *measured outcome* of $\hat{Q}$ is drawn from distribution of eigenvalues $\lambda_{i}$ with probability coefficient of eigenvector $\phi=\sum_{i}c_{i}v_{i}.$
### Expectation ROC
$$
\begin{align}
\frac{\partial}{\partial t}\left< \hat{Q} \right> &=\frac{\partial}{\partial t}\int \Phi^*\hat{Q}\Phi \, dx  \\
&=\int \frac{\partial}{\partial t}\left( \Phi^*\hat{Q}\Phi \right)  \, dx  \\
&=\int \left( \left(\frac{\partial}{\partial t}\Phi^*\right) \hat{Q}\Phi \right)+\left( \Phi^*\frac{\partial}{\partial t}\left( \hat{Q}\Phi \right)  \right)   \, dx  \\
&=\int \left( \left( \frac{1}{i\hbar }\hat{H}\Phi\right)^* \hat{Q}\Phi  \right)  +\frac{1}{i\hbar}\left( \Phi^*\hat{Q}\hat{H}\Phi \right)+\left( \Phi^*\left( \frac{\partial}{\partial t}\hat{Q} \right) \Phi \right)  \, dx  \\
&=\int -\frac{1}{i\hbar}\left(\Phi^*\hat{H}\hat{Q}\Phi\right)  +\frac{1}{i\hbar}\left( \Phi^*\hat{Q}\hat{H}\Phi \right)+\left( \Phi^*\left( \frac{\partial}{\partial t}\hat{Q} \right) \Phi \right)  \, dx  \\
&=\left(\frac{1}{i\hbar}\int \Phi^*[\hat{Q},\hat{H}]\Phi \, dx \right)+\int \Phi^* \frac{\partial\hat{Q}}{\partial t}\Phi \, dx   \\
&=\frac{1}{i\hbar}\left< [\hat{Q},\hat{H}] \right> +\left< \frac{\partial\hat{Q}}{\partial t} \right> .
\end{align}
$$
>[!important] Time-Independent Expectation ROC
> If $\frac{\partial\hat{Q}}{\partial t}=0$ then $$\frac{\partial}{\partial t}\left< \hat{Q} \right> =\frac{1}{i\hbar}\left< [\hat{Q},\hat{H}] \right> .$$

# Problem Solving

>[!important] 
> We want to solve the *energy equation*$$\hat{H}\psi=E\psi,$$i.e. $$\frac{\hbar^{2}}{2m}\nabla^{2}\Psi=V\Psi,$$
> for the *energy eigenstate* $\psi:\mathbb{R}\to \mathbb{C},$ $\hat{H}=-\frac{\hbar^2}{2m}\nabla^{2}+V$ and $E\in \mathbb{R}.$
> Then we get the *stationary state*$$\psi(x,t)=e^{-iEt/\hbar}\psi(x).$$

Wavefunctions are piecewise continuous, and can have Dirac $\delta$.
A *bound state* satisfies $\int \Phi^{2} \, dx$ converges, i.e. it is "real". A *scattering state* is usually $\cos(kx)$ for $x \to \infty.$

Recall that if the potential is finite then the derivative of $\Psi$ must be continuous, i.e. for square well etc. there is a BC for value equality and another BC for derivatives matching up. If $V=\infty$ then we get $\Psi=0$.
## 1D Problem Solving
Our equation is

>[!important] 1D Energy Equation
> $$\psi''+\frac{2m}{\hbar^{2}}(E-V(x))\psi=0.$$
### Free Particle on Circle
On a looped domain $x \in[0,L]$, we get eigenstates $e^{ikx}$, matching boundaries $kL=2\pi n$ and $E_{n}=\frac{{2\pi^{2}\hbar n^{2}}}{mL^{2}}.$ 
### Square Well(s)
Now we have domain $\mathbb{R}$ and experiment with $V(x)$.
#### Infinite case
$$
V=\begin{cases}
0&x \in(0,a) \\
\infty &else
\end{cases}
$$
Then $\Phi=0$ at $else,$ so $\frac{d^2\psi}{dx^2}=-\frac{{2mE}}{\hbar^{2}}\psi.$ Get $\sin(kx)$, check BCs and find $k=\frac{n\pi}{a},$ $E_{n}=\frac{{\pi^{2}\hbar n^{2}}}{2ma^{2}}$ for all $n \in \mathbb{Z}$.
#### Finite case
$$
V=\begin{cases}
-V_{0}&|x| \leq a\\
0 &else
\end{cases}
$$
We want $E \in[-V_{0},0]$ yielding positive KE inside the well, negative KE outside. Then letting $k=\sqrt{ \frac{2m}{\hbar^{2}}\left( V_{0}-|E| \right) }$ and $\kappa=\sqrt{ \frac{{2m|E|}}{\hbar^{2}} },$ we get
$$
\Phi=\begin{cases}
Ae^{\pm ikx}&in\\
Be^{\pm \kappa x} &out
\end{cases}
$$
Higher bound energy $E$ means slower decay $\kappa$ and faster oscillation $k$.
Let $\eta=ka,\xi=\kappa a,$ then cancelling $A,B$ from matching values and $\frac{\partial}{\partial x}$ yields
$$
\begin{align}
\eta^{2}+\xi^{2}&=\frac{{2mV_{0}a^{2}}}{\hbar^{2}},\\
\eta \tan \eta&=\xi.
\end{align}
$$
This yields *finitely* many stationary states. 
### Delta(s)
#### Simple case
$$
V=-V_{0}\delta(x).
$$
Then $\psi''=\frac{2m}{\hbar^{2}}(V_{0}\delta(x)-E)\psi,$ and we must have $E<0$. Integrating near $0$ means
$$
\Delta \psi'|_{0}=V_{0}\frac{2m}{\hbar^{2}}\psi|_{0},
$$
and everywhere else $\psi''=-E\psi.$ We still have to be continuous for $\psi''$ to be defined, so we get $e^{-|kx|}$.
### Simple Harmonic Oscillator
#### Solving Setup
$$
V(x)=\frac{1}{2}m\omega^{2}x^{2}.
$$
This one is a banger. Substitution yields
$$
\psi''=\frac{2m}{\hbar^{2}}\left( \frac{1}{2}m\omega^{2}x^{2}-E \right) \psi.
$$
Take $u=x\sqrt{ \frac{m\omega}{\hbar}, }$ so that letting $\mathcal E=\sqrt{  \frac{2}{\hbar \omega}E}$ yields $$\frac{{\partial^{2}\psi}}{\partial u^{2}}=\left( u^{2} -\mathcal E^{2}\right) \psi.$$
Then plug in $\psi(u)=e^{{-x^{2}}/2}h$ to get $$h''-2uh'+(u^{2}-1)h=(u^{2}-\mathcal E^{2})h,$$
so $h''=2uh'+(1-\mathcal E^{2})h,$ which can be solved in polynomial for arb. degree.
#### Factorization
Let $\hat{a},\hat{a}^*=\left(  \hat{x}\pm \frac{{i \hat{p}}}{m\omega}\right)\sqrt{ \frac{m\omega}{2\hbar} }.$ Then $[a,a^*]=-\frac{2i}{\hbar}\left<  \hat{x},\hat{p}\right>=1.$ 
Recalling $\hat{p}=\frac{\hbar}{i} \frac{\partial}{\partial x},$
$$
\hat{H}=-\frac{\hbar^{2}}{2m} \frac{{\partial^{2}}}{\partial x^{2}}+\frac{1}{2}m\omega^{2}x^{2}=\frac{1}{2}m\omega^{2}\left( x^{2}+ \frac{{\hat{p}^{2}}}{m^{2}\omega^{2}} \right) =\hbar\omega \left( \frac{m\omega}{2\hbar} \right) \left( x^{2}+ \frac{{\hat{p}^{2}}}{m^{2}\omega^{2}} \right)= \hbar\omega \left(a^*a+\frac{1}{2}\right) .
$$
Then the ground solution $\phi_{0}$,
$$
\frac{\hbar\omega}{2}=E_{0}=\left< \phi_{0},E\phi_{0} \right> =\frac{\hbar\omega}{2}+\hbar\omega \left< \hat{a}\phi_{0},\hat{a}\phi_{0} \right>
$$
so $\hat{a}\phi_{0}=0$ everywhere.

Recall that $[\hat{a},\hat{a}^*]=1.$ Let $\hat{N}=\hat{a}^*\hat{a},$ then $\hat{H}=\hat{N}+\frac{1}{2},$ and
$$
[\hat{N},(\hat{a}^*)^{k}]=\hat{a}^{*}\hat{a}(\hat{a}^{*})^{k}-(\hat{a}^{*})^{k}\hat{a}\hat{a}^{*}+(\hat{a}^{*})^{k}=[\hat{N},(\hat{a}^{*})^{k-1}]\hat{a}^{*}+(\hat{a}^{*})^{k}=k(\hat{a}^{*})^{k}.
$$
Similarly for $\hat{a}^{k}$ yields $[\hat N,\hat{a}^k]=-k\hat{a}^k.$

Let $\phi_{k}=(\hat{a}^{*})^{k}\phi_{0},$ we get $$\hat{ N}\phi_{k}=(\hat{N}(\hat{a}^{*})^{k}-(\hat{a}^{*})^{k}\hat{N})\phi_{0}=[\hat{N},(\hat{a}^{*})^{k}]\phi_{0}=k(\hat{a}^{*})^{k}\phi_{0}=k\phi_k.$$
Then $$\hat{H}\phi_{k}=\hbar\omega \left( k+\frac{1}{2} \right) \phi_{k},$$
so $E_{k}=\hbar\omega \left( k+\frac{1}{2} \right).$ Putting it all together:
>[!important] SHO factorization
> Using the *annihilation operator* $\hat{a}=\left( \hat{x}+\frac{{i\hat{p}}}{m\omega} \right)\sqrt{ \frac{{m\omega}}{2\hbar} }$ and the *creation operator* $\hat{a}^{*}=\left( \hat{x}-\frac{{i\hat{p}}}{m\omega} \right)\sqrt{ \frac{{m\omega}}{2\hbar} },$ let $\hat{N}=\hat{a}^{*}\hat{a}.$
> 
> Then given normalized ground $\phi_{0}$, we have:
> $$
> \begin{align}
> [\hat{a},\hat{a}^{*}]&=1,&
> \hat{a}\phi_{0}&=0,\\
> \phi_{{k+1}}&=\frac{{\hat{a}^{*}\phi_{k}}}{\sqrt{ k+1 }}, &
> \phi_{k-1}&=\frac{{\hat{a}\phi_{k}}}{\sqrt{ k }}, \\
> \hat{N}\phi_{k}&=k\phi_{k}, &
> \hat{H}&=\hbar\omega \left( \hat{N}+\frac{1}{2} \right), &
> E_{k}&=\hbar\omega\left( k+\frac{1}{2} \right).
> \end{align}
> $$
