- Non-dimensionalized momentum $\frac{i\hat pa}{\hbar}$ represents location shift; $e^{\frac{i\hat pa}\hbar}=e^{a\frac{\partial}{\partial x}},$ after expansion, $e^{a\frac\partial{\partial x}}\psi(x)=\psi(x+a)$ representing shift left $-a$.

### Angular momentum operator
Typically $\bf L=\bf r\times\bf p.$ We're using central angular momentum with spherical potential, so $\bf r=\bf x, \bf p=\hat p.$
- $\bf\hat L\equiv\bf\hat r\times\bf\hat p$
- $\hat L_x=\hat y\hat p_z-\hat z\hat p_y$
- $\hat L_i$ are Hermitian
- Computing the commutator,
$$
\begin{align*}
[\hat L_x,\hat L_y]
&=[yp_z-zp_y,zp_x-xp_z]\\
&=[yp_z,zp_x]+[zp_y,xp_z]\\
&=y[p_z,z]p_x+x[z,p_z]p_y\\
&=i\hbar(xp_y-yp_x)\\
&=i\hbar L_z.
\end{align*}
$$
- Commutators are ==algebraically cyclic==. Spin operators are similarly algebraically cyclic with commutator.
- Thus no nontrivial eigenstate of $L_x,L_y$ simultaneously exists

- Expanding the original expansion yields $$\hat L_x=\frac\hbar i(y\frac d{dz}-z\frac d{dy})=\frac\hbar i\frac{\partial}{\partial \phi_x}.$$
- Here $\phi_x=\arctan(\frac zy),$ the angle formed by the projection onto the 2D $yz$ plane, with $y$ as base.
- Expressing $L_x,L_y$ using standard spherical $\phi,\theta$ is trickier.

### Radial Ansatz
Working with spherical potential, Schrodinger's becomes an equation in $\bf L^2$ and $\frac d{dr}.$ Now we care about $\psi$ the eigenstate of $\hat L_z,\bf L^2.$ We specify $L_z\psi=\hbar m\psi,{\bf L^2}\psi=\hbar^2l(l+1)\psi.$

Recall $\psi(\theta,\phi)$ is $2\pi$ periodic in both arguments. 

- Solving first directly yields $\frac d{d\phi}\psi=im\psi,$ so $\psi\sim e^{im\phi}.$ by $2\pi$ periodicity $m\in \mathbb Z.$
- Solving second and doing algebra yields $x=\cos\theta,$ $\psi\sim P,$ $$\frac d{dx}\left[(1-x)^2\frac{dP}{dx}\right]+\left[l(l+1)-\frac{m^2}{1-x^2}\right]P=0.$$Here $P$ is Legendre polynomial $l,m$.
- Taking $m=0$, we can solve for coefficients of the series expansion, we get the Legendre polynomials $P_l=\frac1{2^l l!}\left(\frac d{dx}\right)^l(x^2-1)^l.$
- Normalized form is $$Y_{l,m}(\theta,\phi)=\sqrt{\frac{2l+1}{4\pi}\frac{(l-m)!}{(l+m)!}}(-1)^me^{im\phi}P_l^m(\cos\theta),$$with $P_l^m$ above Legendre polynomial.

Resuming with radial ansatz,
- Plugging in $\psi(r,\theta,\phi)=R(r)Y(\theta,\phi)$ yields $u\equiv rR,$ $$-\frac{\hbar^2}{2m}\frac{d^2 u}{dr^2}+\left(V(r)+\frac{\hbar^2l(l+1)}{2mr^2}\right)u=Eu.$$
- We can match singular terms (the $r^{-2}$) as $r\to 0,$ and determine $u\sim r^{l+1}$ in that region.