Typically, Fourier Inversion tells us

$$\hat f(\xi)=\int f(x)e^{-2\pi i\xi x}\,dx\implies f(x)=\int \hat f(\xi)e^{2\pi i\xi x}\,d\xi.$$
If we take $\xi=\frac1{2\pi}k$ then $\hat f(k)=\int f(x)e^{-ikx},$ $f(x)=\frac1{2\pi}\int f(x)e^{ikx}\,dk.$

Splitting this factor and changing things around, we can use

>[!important] QM coordinate space Fourier transform
$$\Psi(x)=\frac1{\sqrt{2\pi}}\int \Phi(x)e^{ikx}\,dk,$$
$$\Phi(k)=\frac1{\sqrt{2\pi}}\int \Psi(x)e^{-ikx}\,dx.$$

Through some interesting manipulation, one can arrive at $\delta(k)=\frac1{2\pi}\int e^{i kx}\,dx.$ Just a broken version of the usual $\delta(\xi)=\int e^{2\pi i x\xi}\,dx.$

Now if we want to rewrite in terms of momentum we do something similar; now $k=\frac1\hbar p,$ so distributing that factor yields

>[!important] QM momentum space Fourier transform
$$\Psi(x)=\frac1{\sqrt{2\pi\hbar}}\int \Phi(p)e^{ipx/\hbar}\,dp,$$
$$\Phi(p)=\frac1{\sqrt{2\pi\hbar}}\int \Psi(x)e^{-ipx/\hbar}\,dx.$$

Then by Parseval/Plancherel's theorem $\int |f|^2\,dx=\int|\hat f|^2\,d\xi,$ we get
$$\int|\Psi|^2\,dx=\int|\Phi|^2\,dp.$$
Then $\Phi$ denotes probability distribution of getting that particular momentum.

If we take the wavenumber interpretation, $\Phi$ becomes distribution of getting that particular wavenumber.

### Expectation
Pretty simple, really.
$$\mathbb E(Q)=\int Q(x)P(x)\,dx=\int Q(x)|\Psi(x)|^2\,dx=\int \Psi^*Q\Psi\,dx.$$
Then we have "joint probabilities" $\langle f|g\rangle$ which is basically $\int f^*g\,dx$.

We denote expectation using $\langle Q\rangle.$ Time derivative plugged into Schrodinger's yields

> [!faq] ROC of Expectation
$$\frac{\partial}{\partial t}\langle Q\rangle=\frac1{i\hbar}\left\langle[\hat Q,\hat H]\right\rangle.$$

## Uncertainty Computation
We can now even plug-and-chug uncertainty, as follows. 

### Proof 1 (smarter)
First note that for arbitrary $u,v$ and constant $t,$ $\int (u+tv)^2=\int u^2+2t\int uv+t^2\int v^2\geq 0,$ so the discriminant in $t$ must be nonpositive i.e. $(2\int uv)^2\leq 4(\int u^2)(\int v^2),$ yielding

>[!c] Cauchy-Schwarz Inequality
>$$\int u^2\int v^2\geq \int uv.$$

Recall that $A$ is *Hermitian* if $\int \phi^*A\psi=\int\psi^*A\phi.$ 

Now let $A_0$ be the expected for $A$, and $B_0$ the same for $B$. 

Assume that $A_0=B_0=0.$ We will not use this condition, and are justified because $\mathbb E[(X-c)^2]$ in general is minimized when $c=\mathbb E[X],$ so we don't lose information by moving the distribution/assuming the mean is $0$ and not using that condition later.

Then $\sigma_A\sigma_b=\langle |A|^2\rangle\langle |B|^2\rangle.$ Note that $\langle |A|^2\rangle=\int \Psi^*A^*A\Psi=\int|A\Psi|^2.$ Then using Cauchy's from above,

$$
\begin{aligned}
\int|A\Psi|^2\int|B\Psi^2|
&\geq\int|A\Psi||B\Psi|\\
&\geq\int\left|\text{Im}((A\Psi)^*B\Psi)\right|\\
&\geq\left|\text{Im}\left(\int(A\Psi)^*B\Psi\right)\right|\\
&=\left|\frac{\int (A\Psi)^*B\Psi - (B\Psi)^*A\Psi}{2i}\right|.
\end{aligned}
$$
Now because $A,B$ are Hermitian,
$$
\begin{aligned}
\left|\frac{\int (A\Psi)^*B\Psi - (B\Psi)^*A\Psi}{2i}\right|
&=\left|\frac{\int \Psi^*BA\Psi-\Psi^*AB\Psi}{2i}\right|\\
&=\left|\frac{\langle [A,B]\rangle}{2}\right|.
\end{aligned}
$$
Thus we've arrived at
>[!important] Robertson Uncertainty
>If $A,B$ are Hermitian operators,
> $$\sigma_A\sigma_B\geq\left|\frac{\langle [A,B]\rangle}{2}\right|. $$

Finally,
$$[\hat x,\hat p]=x\frac\hbar i\frac{\partial}{\partial x}-\frac\hbar i\frac{\partial}{\partial x} x=-\frac\hbar i=\hbar i.$$
Therefore,

>[!important] Heisenberg Uncertainty
> $$\sigma_x\sigma_p\geq\frac\hbar 2.$$


### Proof 2 (dumber)
As before, note that $\sigma_A=\int\Psi^*(A-A_0)^2\Psi=\int\Psi^*(A-A_0)^*(A-A_0)\Psi=\int|(A-A_0)\Psi)|^2.$ 

Assume that $\Psi(x),\Phi(p)$ are 0-meaned. Then $\sigma_x^2=\langle x\Psi(x)\mid x\Psi(x)\rangle,$ and $\sigma_p^2=\int p|\Phi(p)|^2\,dp.$ Note that by Parseval's, $\int p|\Phi(p)|^2\,dp=\langle\mathcal F^{-1}(p\Phi(p))\mid\mathcal F^{-1}(p\Phi(p))\rangle,$ so now we compute this function using *integration by parts.*

First 
$$
\begin{aligned}
p\Phi(p)\sqrt{2\pi\hbar}
&=\int p\Psi(x)e^{-ipx/\hbar}\,dx\\
&=\left.i\hbar\Psi(x)e^{-ipx/\hbar}\right|_{-\infty}^{\infty} - i\hbar\int\frac{\partial\Psi}{\partial x}e^{-ipx/\hbar}\,dx\\
&=-i\hbar\int\frac{\partial\Psi}{\partial x}e^{-ipx/\hbar}\,dx.
\end{aligned}
$$
Then
$$
\begin{aligned}
\mathcal F^{-1}(p\Phi(p))(x)
&=\frac1{\sqrt{2\pi\hbar}}\int p\Phi(p)e^{ipx/\hbar}\,dp\\
&=\frac1{2\pi\hbar}\int e^{ipx/\hbar}\,dp(-i\hbar)\int\frac{\partial\Psi}{\partial x'}e^{-ipx'/\hbar}\,dx'\\
&=\frac1{2\pi i}\int \frac{\partial\Psi}{\partial x'}\,dx'\int e^{\frac{ip(x-x')}\hbar}\,dp\\
&=\frac{\hbar}i\frac{\partial\Psi}{\partial x}\\
&=\hat p\Psi(x).
\end{aligned}
$$
Finally,
$$
\begin{aligned}
\sigma_x^2\sigma_p^2
&= \langle x\Psi(x)\mid x\Psi(x)\rangle\langle \hat p\Psi(x)\mid\hat p\Psi(x)\rangle\\
&\geq |\langle x\Psi(x)\mid\hat p\Psi(x)\rangle|^2\\
&\geq \left(\frac{\langle x\Psi(x)\mid \hat p\Psi(x)\rangle-\langle \hat p\Psi(x)\mid x\Psi(x)\rangle}{2i}\right)^2.
\end{aligned}
$$
Then (because of magic and how self-adjoint operators like $\hat p$ work)
$$
\begin{aligned}
\langle x\Psi(x)\mid\hat p\Psi(x)\rangle-\langle\hat p\Psi(x)\mid x\Psi(x)\rangle
&=\langle x\Psi(x)\mid\hat p\Psi(x)\rangle-\langle\Psi(x)\mid \hat p(x\Psi(x))\rangle\\
&=\int x\Psi^*\frac\hbar i\Psi'-\Psi^*\frac\hbar{i}\frac{\partial}{\partial x}(x\Psi)\,dx\\
&=\frac\hbar i\int -\Psi\Psi^*\,dx\\
&=\hbar i.
\end{aligned}
$$
Thus $\sigma_x^2\sigma_p^2\geq \left(\frac{\hbar}2\right)^2$ and $\sigma_x\sigma_p\geq\frac\hbar2.$